idk

theories/Semantics.v
@@ -1,6 +1,7 @@
 From Coq Require Import Strings.String.
 From Coq Require Import Lists.List.
 From Coq Require Import Init.Nat.
+From Coq Require Import Program.Wf.
 
 Require Import Syntax. Import Syntax.
 
@@ -23,15 +24,17 @@ Module Semantics.
   Inductive Env : Type :=
   | EmptyEnv : Env
   | ExtendEnv : string -> Value -> Env -> Env
-    with Value : Type :=
-    | V_Nat : nat -> Value
-    | V_Bool : bool -> Value
-    | V_Closure : string -> FExpr_Sub -> Env -> Value
-    | V_ReturnValue : Value -> Value.
+
+  with Value : Type :=
+  | V_Nat : nat -> Value
+  | V_Bool : bool -> Value
+  | V_Closure : string -> FExpr_Sub -> Env -> Value
+  | V_Fix : string -> FExpr_Sub -> Env -> Value.
 
   Fixpoint lookup_env (varName : string) (env : Env) {struct env} : sum string Value :=
     match env with
-    | EmptyEnv => inl ("(lookup_env) Error: Unbound variable '" ++ varName ++ "'")
+    | EmptyEnv =>
+        inl ("(lookup_env) Error: Unbound variable '" ++ varName ++ "'")
     | ExtendEnv name value restEnv =>
         if String.eqb varName name
         then inr value
@@ -62,30 +65,43 @@ Module Semantics.
       match expr with
       | F_Var varName =>
           match lookup_env varName env with
-          | inr value =>
-              inr value
+          | inr (V_Closure name expr env) =>
+              inr (V_Closure name expr env)
+          | inr (V_Fix name expr env) =>
+              inr (V_Fix name expr env)
+          | inr _ =>
+              inl
+                (("(Feval_Sub) Error: Variable does not resolve to a function '" ++ varName ++ "'") :: nil)
           | inl err =>
               inl
                 (("(Feval_Sub) Error: Unbound variable '" ++ varName ++ "'") :: err :: nil)
           end
       | F_Lambda paramName bodyExpr =>
-          inr (V_Closure paramName bodyExpr env)
+          inr (V_Closure paramName (F_Lambda paramName bodyExpr) env)
+      | F_Fix fixName (F_Lambda paramName bodyExpr) => 
+          let fixClosure := V_Fix fixName (F_Lambda paramName bodyExpr) env in
+          let env' := ExtendEnv fixName fixClosure env in
+          inr fixClosure (* Wrap the result in a closure *)
+      | F_Fix fixName _ =>
+          inl
+            (("(Feval_Sub) Error: Fix expression does not resolve to a function '" ++ fixName ++ "'") :: nil)
       | F_Apply funcExpr argExpr =>
           match Feval_Sub funcExpr env max' with
-          | inr (V_Closure paramName bodyExpr env) =>
-              let argValueSum := Feval_Sub argExpr env max' in
-              match argValueSum with
+          | inr (V_Closure _ (F_Lambda paramName bodyExpr) closureEnv) =>
+              match Feval_Sub argExpr env max' with
               | inr argValue =>
-                let extendedEnv := ExtendEnv paramName argValue env in
-                Feval_Sub bodyExpr extendedEnv max'
+                Feval_Sub bodyExpr (ExtendEnv paramName argValue closureEnv) max'
               | inl err =>
-                  inl
-                    ("(Feval_Sub) Error: Function argument did not evaluate to a value"
-                      :: err)
+                  inl 
+                    ("Error: Function argument did not evaluate to a value" :: err)
               end
+          | inr (V_Fix fixName (F_Lambda paramName bodyExpr) fixEnv) =>
+              let fixClosure := V_Fix fixName (F_Lambda paramName bodyExpr) fixEnv in
+              let env' := ExtendEnv fixName fixClosure env in
+              Feval_Sub bodyExpr env' max'
           | _ =>
               inl
-                ("(Feval_Sub) Error: Function did not evaluate to a closure" :: nil)
+                ("Error: Attempted to apply a non-function" :: nil)
           end
       | F_Cond condExpr trueExpr falseExpr =>
           match Beval condExpr env max' with
@@ -136,29 +152,9 @@ Module Semantics.
           match Feval_Sub f env max' with
           | inr (V_Nat n) =>
               inr n
-          | inr (V_Bool b) =>
+          | _ =>
               inl
-                ("(Aeval) Error: Function did not evaluate to a number: 'V_Bool " ++ (bool_to_string b) ++ "'")
-          | inr (V_Closure name _ _) =>
-              inl
-                ("(Aeval) Error: Function did not evaluate to a number: 'V_Closure " ++ name ++ "'")
-          | inr (V_ReturnValue val) =>
-              match val with
-              | V_Nat n =>
-                  inr n
-              | V_Bool b =>
-                  inl
-                    ("(Aeval) Error: Function did not evaluate to a number: 'V_Bool " ++ (bool_to_string b) ++ "'")
-              | V_Closure name _ _ =>
-                  inl
-                    ("(Aeval) Error: Function did not evaluate to a number: 'V_Closure " ++ name ++ "'")
-              | V_ReturnValue _ =>
-                  inl
-                    "(Aeval) Error: Function did not evaluate to a number: 'V_ReturnValue'"
-              end
-          | inl err =>
-              inl
-              ("(Aeval) Error: Function did not evaluate to a number: " ++ concat_string_list err)
+                "(Aeval) Error: Function did not evaluate to a number"
           end
       | A_Var varName =>
           match lookup_env varName env with
@@ -208,27 +204,79 @@ Module Semantics.
                 ("(Beval) Error: Variable did not evaluate to a boolean: '" ++ varName ++ "'")
           end
       end
+    end
+
+  with fix100 (f : Value) (max : nat) : sum (list string) Value :=
+    match max with
+    | 0 =>
+        inl
+          ("(fix) Error: Maximum recursion depth exceeded" :: nil)
+    | S max' =>
+      match f with
+      | V_Fix var expr env =>
+          Feval_Sub expr (ExtendEnv var (V_Fix var expr env) env) max'
+      | _ =>
+          inl
+            ("(fix) Error: Value is not a fixpoint" :: nil)
+      end
     end.
 
-  Definition Feval (expr : FExpr) (env : Env) (max : nat) : sum (list string) Value :=
-    match expr with
-    | F_Let varName bindExpr bodyExpr =>
-        let extendedEnv := ExtendEnv varName (V_Closure varName bindExpr env) env in
-        match Feval_Sub bindExpr extendedEnv max with
-        | inr val =>
-            Feval_Sub bodyExpr (ExtendEnv varName val env) max
-        | inl err =>
-            inl err
-        end
+  Fixpoint Feval (expr : FExpr) (env : Env) (max : nat) : sum (list string) Value :=
+    match max with
+    | 0 =>
+        inl
+          ("(Feval) Error: Maximum recursion depth exceeded" :: nil)
+    | S max' =>
+      match expr with
+      | F_Let varName bindExpr bodyExpr =>
+          match Feval_Sub bindExpr env max' with
+          | inr val =>
+              Feval_Sub bodyExpr (ExtendEnv varName val env) max'
+          | inl err =>
+              inl err
+          end
+      | F_LetRec varname bindExpr bodyExpr =>
+          Feval (F_Let varname (F_Fix varname bindExpr) bodyExpr) env max'
+      end
     end.
 
-  Compute Feval          (F_Let "factorial"
-            (F_Lambda "n"
-               (F_Cond (B_Eq (E_Arith (A_Var "n")) (E_Arith (A_Const 1)))
-                  (F_Return (E_Arith (A_Const 1)))
-                  (F_Apply (F_Var "factorial")
-                     (F_Return (E_Arith (A_Sub (A_Var "n") (A_Const 1)))))))
-            (F_Apply (F_Var "factorial") (F_Return (E_Arith (A_Var "input"))))) (ExtendEnv "input" (V_Nat 5) EmptyEnv) 100.
+  Compute Beval (B_Eq (E_Arith (A_Const 3)) (E_Arith (A_Const 1))) EmptyEnv 1000.
+
+  Compute
+    Feval
+      (F_LetRec "factorial"
+        (F_Lambda "n"
+          (F_Cond (B_Eq (E_Arith (A_Var "n")) (E_Arith (A_Const 1)))
+            (F_Return (E_Arith (A_Const 1)))
+              (F_Apply
+                (F_Var "factorial")
+                (F_Return (E_Arith (A_Var "n")))
+            )
+          )
+        )
+          (F_Var "factorial")
+      )
+      (ExtendEnv "input" (V_Nat 5) EmptyEnv)
+      1000.
+
+  Compute
+    Feval_Sub
+    (F_Apply
+    (F_Fix "factorial"
+      (F_Lambda "n"
+        (F_Cond
+          (B_Eq (E_Arith (A_Func (F_Var "n"))) (E_Arith (A_Const 1)))
+          (F_Return ((E_Arith (A_Const 1))))
+          (F_Return (E_Arith
+            (A_Mul
+              (A_Func (F_Var "n"))
+              (A_Func (F_Apply
+                (F_Var "factorial")
+                (F_Return (E_Arith (A_Sub (A_Func (F_Var "n")) (A_Const 1))))
+              ))))))))
+              (F_Return (E_Arith (A_Const 5)))
+              ) EmptyEnv 1000.
+
 
 
   Compute Feval_Sub ((F_Return (E_Arith (A_Add (A_Const 1) (A_Const 2))))) EmptyEnv 100.
